<?xml version="1.0" encoding="UTF-8"?>

<exercises>

  <exercise>
    <statement>
      <p> If a matrix <m>A</m> is invertible, there is a sequence of
      row operations that transforms <m>A</m> into the
      identity matrix <m>I</m>.  We have seen that every row operation can be
      performed by matrix multiplication.  If the <m>j^{th}</m> step
      in the Gaussian elimination process is performed by multiplying
      by <m>E_j</m>, then we have
      <me>
	E_p\cdots E_2E_1 A = I
      </me>,
      which means that
      <me>
	A^{-1} = E_p\cdots E_2E_1
      </me>.
      For each of the following matrices, find a sequence of row
      operations that transforms the matrix to the identity <m>I</m>.
      Write the matrices <m>E_j</m> that perform the steps and use
      them to find <m>A^{-1}</m>.
      <ol marker="a.">
	<li><p>
	  <me>A = \left[\begin{array}{rrr}
	  0 \amp 2 \amp 0 \\
	  -3 \amp 0 \amp 0 \\
	  0 \amp 0 \amp 1 \\
	  \end{array}\right]
	  </me>.
	</p></li>

      	<li><p>
	  <me>A = \left[\begin{array}{rrrr}
	  1 \amp 0 \amp 0 \amp 0 \\
	  2 \amp 1 \amp 0 \amp 0 \\
	  0 \amp -3 \amp 1 \amp 0 \\
	  0 \amp 0 \amp 2 \amp 1 \\
	  \end{array}\right]
	  </me>.
	</p></li>

	<li><p>
	  <me>A = \left[\begin{array}{rrr}
	  1 \amp 1 \amp 1 \\
	  0 \amp 1 \amp 1 \\
	  0 \amp 0 \amp 2 \\
	  \end{array}\right]
	  </me>.
	</p></li>

      </ol></p>
    </statement>

    <solution>
      <p><ol marker="a.">
	<li><p>
	  If
	  <me>
	    P =
	    \left[\begin{array}{rrr}
	    0 \amp 1 \amp 0 \\
	    1 \amp 0 \amp 0 \\
	    0 \amp 0 \amp 1 \\
	    \end{array}\right],
	    S_1 =
	    \left[\begin{array}{rrr}
	    -\frac13 \amp 0 \amp 0 \\
	    0 \amp 1 \amp 0 \\
	    0 \amp 0 \amp 1 \\
	    \end{array}\right],
	    S_2 =
	    \left[\begin{array}{rrr}
	    1 \amp 0 \amp 0 \\
	    0 \amp \frac12 \amp 0 \\
	    0 \amp 0 \amp 1 \\
	    \end{array}\right]\text{,}
	  </me>
	  then <m>S_2S_1P A = I</m> so that <m>A^{-1}=S_2S_1P=
	  \left[\begin{array}{rrr}
	  0 \amp -\frac13 \amp 0 \\
	  \frac12 \amp 0 \amp 0 \\
	  0 \amp 0 \amp 1 \\
	  \end{array}\right]
	  </m>.
	</p></li>

	<li><p>
	  We use three replacement operations
	  <me>
	    \begin{array}{l}
	    L_1 =
	    \left[\begin{array}{rrrr}
	    1 \amp 0 \amp 0 \amp 0 \\
	    -2 \amp 1 \amp 0 \amp 0 \\
	    0 \amp 0 \amp 1 \amp 0 \\
	    0 \amp 0 \amp 0 \amp 1 \\
	    \end{array}\right],
	    L_2 =
	    \left[\begin{array}{rrrr}
	    1 \amp 0 \amp 0 \amp 0 \\
	    0 \amp 1 \amp 0 \amp 0 \\
	    0 \amp 3 \amp 1 \amp 0 \\
	    0 \amp 0 \amp 0 \amp 1 \\
	    \end{array}\right], \\
	    L_3 =
	    \left[\begin{array}{rrrr}
	    1 \amp 0 \amp 0 \amp 0 \\
	    0 \amp 1 \amp 0 \amp 0 \\
	    0 \amp 0 \amp 1 \amp 0 \\
	    0 \amp 0 \amp -2 \amp 1 \\
	    \end{array}\right]\text{.}
	    \end{array}
	  </me>
	  Therefore, <m>L_3L_2L_1A = I</m> so <m>A^{-1} = L_3L_2L_1 =
	    \left[\begin{array}{rrrr}
	    1 \amp 0 \amp 0 \amp 0 \\
	    -2 \amp 1 \amp 0 \amp 0 \\
	    -6 \amp 3 \amp 1 \amp 0 \\
	    12 \amp -6 \amp -2 \amp 1 \\
	    \end{array}\right]
	  </m>.
	</p></li>

	<li><p>
	  We use a scaling followed by replacement operations:
	  <me>
	    S =
	    \left[\begin{array}{rrr}
	    1 \amp 0 \amp 0 \\
	    0 \amp 1 \amp 0 \\
	    0 \amp 0 \amp \frac12 \\
	    \end{array}\right],
	    U_1 =
	    \left[\begin{array}{rrr}
	    1 \amp 0 \amp -1 \\
	    0 \amp 1 \amp -1 \\
	    0 \amp 0 \amp 1 \\
	    \end{array}\right],
	    U_2 = \begin{bmatrix}
	    1 \amp 0 \amp -1 \\
	    0 \amp 1 \amp 0 \\
	    0 \amp 0 \amp 1 \\
	    \end{bmatrix},
	    U_3 = 
	    \left[\begin{array}{rrr}
	    1 \amp -1 \amp 0 \\
	    0 \amp 1 \amp 0 \\
	    0 \amp 0 \amp 1 \\
	    \end{array}\right]\text{.}
	  </me>
	  This gives <m>U_3U_2U_1SA = I</m> so that
	  <m>
	    A^{-1} = U_3U_2U_1S =
	    \left[\begin{array}{rrr}
	    1 \amp -1 \amp 0 \\
	    0 \amp 1 \amp -\frac12 \\
	    0 \amp 0 \amp \frac12 \\
	    \end{array}\right]
	    </m>.
	</p></li>
      </ol></p>
    </solution>

    <answer>
      <p><ol marker="a.">
	<li><p>
	  <m>A^{-1}=
	  \left[\begin{array}{rrr}
	  0 \amp -\frac13 \amp 0 \\
	  \frac12 \amp 0 \amp 0 \\
	  0 \amp 0 \amp 1 \\
	  \end{array}\right]
	  </m>.
	</p></li>

	<li><p>
	  <m>A^{-1} = 
	    \left[\begin{array}{rrrr}
	    1 \amp 0 \amp 0 \amp 0 \\
	    -2 \amp 1 \amp 0 \amp 0 \\
	    -6 \amp 3 \amp 1 \amp 0 \\
	    12 \amp -6 \amp -2 \amp 1 \\
	    \end{array}\right]
	  </m>.
	</p></li>

	<li><p>
	  <m>
	    A^{-1} = 
	    \left[\begin{array}{rrr}
	    1 \amp -1 \amp 0 \\
	    0 \amp 1 \amp -\frac12 \\
	    0 \amp 0 \amp \frac12 \\
	    \end{array}\right]
	    </m>.
	</p></li>
      </ol></p>
    </answer>
    
  </exercise>

  <exercise>
    <statement>
      <p>
	Suppose that we start with the <m>3\by3</m> matrix <m>A</m>,
	perform the following sequence of row operations:
	<ol marker="1.">
	  <li><p>  Multiply row 1 by -2 and add to row 2. </p></li>
	  <li><p>  Multiply row 1 by 4 and add to row 3. </p></li>
	  <li><p>  Scale row 2 by <m>1/2</m>. </p></li>
	  <li><p>  Multiply row 2 by -1 and add to row 3, </p></li>
	</ol>
	and arrive at the upper triangular matrix
	<me>
	  U = \left[\begin{array}{rrr}
	  3 \amp 2 \amp -1 \\
	  0 \amp 1 \amp 3 \\
	  0 \amp 0 \amp -4 \\
	  \end{array}\right].
	</me>
	<sage language="python">
	  <input>
	  </input>
	</sage>
	<ol marker="a.">
	  <li><p> Write the matrices <m>E_1</m>, <m>E_2</m>,
	  <m>E_3</m>, and <m>E_4</m> that perform the four row
	  operations. </p></li>

	  <li><p> 
	  Find the
	  matrix <m>E = E_4E_3E_2E_1</m>. </p></li>

	  <li><p> We then have <m>E_4E_3E_2E_1 A = EA = U</m>.  Now
	  that we have the matrix <m>E</m>, find the original matrix
	  <m>A = E^{-1}U</m>.
	  </p></li>
	</ol>
      </p>
    </statement>

    <solution>
      <p><ol marker="a.">
	<li><p>
	  We have
	  <me>
	    \begin{array}{cc}
	    E_1=\left[\begin{array}{rrr}
	    1 \amp 0 \amp 0 \\
	    -2 \amp 1 \amp 0 \\
	    0 \amp 0 \amp 1
	    \end{array}\right],
	    \amp
	    E_2=\left[\begin{array}{rrr}
	    1 \amp 0 \amp 0 \\
	    0 \amp 1 \amp 0 \\
	    4 \amp 0 \amp 1
	    \end{array}\right], \\
	    E_3 = \left[\begin{array}{rrr}
	    1 \amp 0 \amp 0 \\
	    0 \amp \frac{1}{2} \amp 0 \\
	    0 \amp 0 \amp 1
	    \end{array}\right],
	    \amp
	    E_4 = 
	    \left[\begin{array}{rrr}
	    1 \amp 0 \amp 0 \\
	    0 \amp 1 \amp 0 \\
	    0 \amp -1 \amp 1
	    \end{array}\right]\text{.}
	    \end{array}
	  </me>
	</p></li>

	<li><p>
	  We have
	  <m> E = E_4E_3E_2E_1 = 
	  \left[\begin{array}{rrr}
	  1 \amp 0 \amp 0 \\
	  -1 \amp \frac{1}{2} \amp 0 \\
	  5 \amp -\frac12 \amp 1
	  \end{array}\right]
	  </m>.
	</p></li>

	<li><p>
	  We write <m>A=E^{-1}U=
	  \left[\begin{array}{rrr}
	  3 \amp 2 \amp -1 \\
	  6 \amp 6 \amp 4 \\
	  -12 \amp -7 \amp 3
	  \end{array}\right]
	  </m>.
	</p></li>
      </ol></p>
    </solution>
    
    <answer>
      <p><ol marker="a.">
	<li><p>
	  We have
	  <me>
	    \begin{array}{cc}
	    E_1=\left[\begin{array}{rrr}
	    1 \amp 0 \amp 0 \\
	    -2 \amp 1 \amp 0 \\
	    0 \amp 0 \amp 1
	    \end{array}\right],
	    \amp
	    E_2=\left[\begin{array}{rrr}
	    1 \amp 0 \amp 0 \\
	    0 \amp 1 \amp 0 \\
	    4 \amp 0 \amp 1
	    \end{array}\right], \\
	    E_3 = \left[\begin{array}{rrr}
	    1 \amp 0 \amp 0 \\
	    0 \amp \frac{1}{2} \amp 0 \\
	    0 \amp 0 \amp 1
	    \end{array}\right],
	    \amp
	    E_4 = 
	    \left[\begin{array}{rrr}
	    1 \amp 0 \amp 0 \\
	    0 \amp 1 \amp 0 \\
	    0 \amp -2 \amp 1
	    \end{array}\right]\text{.}
	    \end{array}
	  </me>
	</p></li>

	<li><p>
	  <m> E = 
	  \left[\begin{array}{rrr}
	  1 \amp 0 \amp 0 \\
	  -1 \amp \frac{1}{2} \amp 0 \\
	  6 \amp -1 \amp 1
	  \end{array}\right]
	  </m>.
	</p></li>

	<li><p>
	  <m>A=
	  \left[\begin{array}{rrr}
	  3 \amp 2 \amp -1 \\
	  6 \amp 6 \amp 4 \\
	  -12 \amp -6 \amp 6
	  \end{array}\right]
	  </m>.
	</p></li>
      </ol></p>
    </answer>
    
  </exercise>


</exercises>
